Rewrote the module for generator. Add in defined generator with state. Remove dependency on LLVMEvents

src/coq/QC/GenAlive2.v
@@ -14,6 +14,7 @@ From ExtLib.Structures Require Export
 
 Require Import ExtLib.Data.Monads.StateMonad.
 Require Import ExtLib.Structures.Monads.
+Require Import ExtLib.Data.Monads.EitherMonad.
 Require Export ExtLib.Structures.Functor.
 
 Require Import List.
@@ -74,47 +75,239 @@ Set Warnings "-extraction-opaque-accessed,-extraction".
 (*     end. *)
 (* End GEN_ALIVE2'. *)
 
-Module GEN_ALIVE2 (ADDR : MemoryAddress.ADDRESS) (IP:MemoryAddress.INTPTR) (SIZEOF : Sizeof) (LLVMEvents:LLVM_INTERACTIONS(ADDR)(IP)(SIZEOF)).
-  Import LLVMEvents.
-  Import DV.
+(* Module GEN_ALIVE2 (ADDR : MemoryAddress.ADDRESS) (IP:MemoryAddress.INTPTR) (SIZEOF : Sizeof) (LLVMEvents:LLVM_INTERACTIONS(ADDR)(IP)(SIZEOF)). *)
+(*   Import LLVMEvents. *)
+(*   Import DV. *)
+
+(*   Record GenState := { *)
+(*     num_void : nat}. *)
+
+(*   Definition init_GenState : GenState *)
+(*     := *)
+(*     {| *)
+(*       num_void := 0 *)
+(*     |}. *)
+(*   (* {}. *) *)
+    
+(*   Definition GenALIVE2 := (eitherT string (stateT GenState G)). *)
+
+(*   #[global] Instance monad_stateT {s m} `{Monad m} : Monad (stateT s m). *)
+(*   Proof. *)
+(*     apply Monad_stateT. typeclasses eauto. *)
+(*   Defined. *)
+
+(*   #[global] Instance STGST : Monad (stateT GenState G). *)
+(*   Proof. *)
+(*     apply Monad_stateT. typeclasses eauto. *)
+(*   Defined. *)
   
-  Fixpoint gen_uvalue `{MonadExc string G} (t : typ): G uvalue :=
+(*   #[global] Instance MGEN : Monad GenALIVE2. *)
+(*   Proof. *)
+(*     apply Monad_eitherT. typeclasses eauto. *)
+(*   Defined. *)
+
+(*   Definition lift_GenALIVE2 {A} (g : G A) : GenALIVE2 A. *)
+(*     unfold GenALIVE2. *)
+(*     apply mkEitherT. *)
+(*     apply mkStateT. *)
+(*     refine (fun stack => _). *)
+(*     refine (a <- g;; _). *)
+(*     refine (ret (inr a, stack)). *)
+(*   Defined. *)
+
+(*   #[global] Instance MGENT: MonadT GenALIVE2 G. *)
+(*   unfold GenALIVE2. *)
+(*   constructor. *)
+(*   exact @lift_GenALIVE2. *)
+(*   Defined. *)
+  
+(*   Definition failGen {A : Type} (s : string) : GenALIVE2 A. *)
+(*     apply mkEitherT. *)
+(*     apply mkStateT. *)
+(*     refine (fun stack => _ ). *)
+(*     exact (ret (inl (s), stack)). *)
+(*   Defined. *)
+
+(*   Definition vectorOf_ALIVE2 {A : Type} (k : nat) (g : GenALIVE2 A) : GenALIVE2 (list A). *)
+(*     refine (fold_left _ _ _). *)
+(*     refine (fun l g => _). *)
+(*     refine (a <- g ;; _). *)
+(*     refine (a' <- l ;; _). *)
+(*     exact (ret (a :: a')). *)
+(*     exact (repeat g k). *)
+(*     exact (ret []). *)
+(*   Defined. *)
+
+(*   Definition run_GenALIVE2 {A : Type} (g : GenALIVE2 A) : G (string + A) *)
+(*     := *)
+(*     let ran := runStateT (unEitherT g) init_GenState in *)
+(*     '(errA, _) <- ran;; *)
+(*     ret errA *)
+(*   . *)
+  
+(*   Fixpoint gen_uvalue (t : typ) : GenALIVE2 uvalue := *)
+(*     match t with *)
+(*     | TYPE_I i => *)
+(*         match i with *)
+(*         | 1%N => *)
+(*             ret UVALUE_I1 <*> (ret repr <*> lift_GenALIVE2 (choose (0, 1))) *)
+(*         | 8%N => *)
+(*             ret UVALUE_I8 <*> (ret repr <*> lift_GenALIVE2 (choose (0, 2^8 - 1))) *)
+(*         | 32%N => *)
+(*             ret UVALUE_I32 <*> (ret repr <*> lift_GenALIVE2 (choose (0, 2^32 - 1))) *)
+(*         | 64%N => *)
+(*             ret UVALUE_I64 <*> (ret repr <*> lift_GenALIVE2 (choose (0, 2^64 - 1))) *)
+(*         | _ => *)
+(*             failGen "Invalid size" *)
+(*         end *)
+(*     | TYPE_Float => *)
+(*         ret UVALUE_Float <*> lift_GenALIVE2 fing32 *)
+(*     | TYPE_Double => *)
+(*         failGen "Generating UValue Double - Not supported" *)
+(*     | TYPE_Void => ret UVALUE_None *)
+(*     | TYPE_Vector sz subtyp => *)
+(*         ret UVALUE_Vector <*> (vectorOf_ALIVE2 (N.to_nat sz) (gen_uvalue subtyp)) *)
+(*     | TYPE_Array sz subtyp => *)
+(*         ret UVALUE_Array <*> (vectorOf_ALIVE2 (N.to_nat sz) (gen_uvalue subtyp)) *)
+(*     | _ => failGen "Invalid" *)
+(*     end. *)
+(* End GEN_ALIVE2. *)
+
+Module GEN_ALIVE2 (ADDR : MemoryAddress.ADDRESS) (IP:MemoryAddress.INTPTR) (SIZEOF : Sizeof).
+  Module DV := DynamicValues.DVALUE(ADDR)(IP)(SIZEOF).
+  Import DV.
+  Record GenState := {
+    num_void : nat}.
+
+  Definition init_GenState : GenState
+    :=
+    {|
+      num_void := 0
+    |}.
+  (* {}. *)
+    
+  Definition GenALIVE2 := (eitherT string (stateT GenState G)).
+
+  #[global] Instance monad_stateT {s m} `{Monad m} : Monad (stateT s m).
+  Proof.
+    apply Monad_stateT. typeclasses eauto.
+  Defined.
+
+  #[global] Instance STGST : Monad (stateT GenState G).
+  Proof.
+    apply Monad_stateT. typeclasses eauto.
+  Defined.
+  
+  #[global] Instance MGEN : Monad GenALIVE2.
+  Proof.
+    apply Monad_eitherT. typeclasses eauto.
+  Defined.
+
+  Definition lift_GenALIVE2 {A} (g : G A) : GenALIVE2 A.
+    unfold GenALIVE2.
+    apply mkEitherT.
+    apply mkStateT.
+    refine (fun stack => _).
+    refine (a <- g;; _).
+    refine (ret (inr a, stack)).
+  Defined.
+
+  #[global] Instance MGENT: MonadT GenALIVE2 G.
+  unfold GenALIVE2.
+  constructor.
+  exact @lift_GenALIVE2.
+  Defined.
+  
+  Definition failGen {A : Type} (s : string) : GenALIVE2 A.
+    apply mkEitherT.
+    apply mkStateT.
+    refine (fun stack => _ ).
+    exact (ret (inl (s), stack)).
+  Defined.
+
+  Definition vectorOf_ALIVE2 {A : Type} (k : nat) (g : GenALIVE2 A) : GenALIVE2 (list A).
+    refine (fold_left _ _ _).
+    refine (fun l g => _).
+    refine (a <- g ;; _).
+    refine (a' <- l ;; _).
+    exact (ret (a :: a')).
+    exact (repeat g k).
+    exact (ret []).
+  Defined.
+
+  Definition run_GenALIVE2 {A : Type} (g : GenALIVE2 A) : G (string + A)
+    :=
+    let ran := runStateT (unEitherT g) init_GenState in
+    '(errA, _) <- ran;;
+    ret errA
+  .
+  
+  Fixpoint gen_uvalue (t : typ) : GenALIVE2 uvalue :=
     match t with
     | TYPE_I i =>
         match i with
         | 1%N =>
-            returnGen UVALUE_I1 <*> (returnGen repr <*> (choose (0, 1)))
-            (* x <- choose (0,1);; *)
-            (* returnGen (UVALUE_I1 (repr x))  *)
+            ret UVALUE_I1 <*> (ret repr <*> lift_GenALIVE2 (choose (0, 1)))
         | 8%N =>
-            returnGen UVALUE_I8 <*> (returnGen repr <*> (choose (0, 2^8)))
-            (* x <- choose (0,2 ^ 8);; *)
-            (* returnGen (UVALUE_I8 (repr x)) *)
+            ret UVALUE_I8 <*> (ret repr <*> lift_GenALIVE2 (choose (0, 2^8 - 1)))
         | 32%N =>
-            returnGen UVALUE_I32 <*> (returnGen repr <*> (choose (0, 2^32)))
-            (* x <- choose (0, 2 ^ 32);; *)
-            (* returnGen (UVALUE_I32 (repr x)) *)
+            ret UVALUE_I32 <*> (ret repr <*> lift_GenALIVE2 (choose (0, 2^32 - 1)))
         | 64%N =>
-            returnGen UVALUE_I64 <*> (returnGen repr <*> (choose (0, 2^64)))
-            (* x <- choose (0, 2 ^ 63);; *)
-            (* returnGen (UVALUE_I64 (repr x)) *)
-        | _ => failwith "Invalid size"
+            ret UVALUE_I64 <*> (ret repr <*> lift_GenALIVE2 (choose (0, 2^64 - 1)))
+        | _ =>
+            failGen "Invalid size"
         end
     | TYPE_Float =>
-        returnGen UVALUE_Float <*> fing32
+        ret UVALUE_Float <*> lift_GenALIVE2 fing32
     | TYPE_Double =>
-        returnGen UVALUE_None (* FailGen *)
-    | TYPE_Void => returnGen UVALUE_None
+        failGen "Generating UValue Double - Not supported"
+    | TYPE_Void => ret UVALUE_None
     | TYPE_Vector sz subtyp =>
-        returnGen UVALUE_Vector <*> vectorOf (N.to_nat sz) (gen_uvalue subtyp)
+        ret UVALUE_Vector <*> (vectorOf_ALIVE2 (N.to_nat sz) (gen_uvalue subtyp))
     | TYPE_Array sz subtyp =>
-        returnGen UVALUE_Array <*> vectorOf (N.to_nat sz) (gen_uvalue subtyp)
-    | _ => failwith "Unimplemented uvalue generators"
+        ret UVALUE_Array <*> (vectorOf_ALIVE2 (N.to_nat sz) (gen_uvalue subtyp))
+    | _ => failGen "Invalid"
     end.
+                                            
+
+  
+  (* Fixpoint gen_uvalue (t : typ): GenALIVE2 uvalue := *)
+  (*   match t with *)
+  (*   | TYPE_I i => *)
+  (*       match i with *)
+  (*       | 1%N => *)
+  (*           ret UVALUE_I1 <*> (returnGen repr <*> (choose (0, 1))) *)
+  (*           (* x <- choose (0,1);; *) *)
+  (*           (* returnGen (UVALUE_I1 (repr x))  *) *)
+  (*       | 8%N => *)
+  (*           ret UVALUE_I8 <*> (returnGen repr <*> (choose (0, 2^8))) *)
+  (*           (* x <- choose (0,2 ^ 8);; *) *)
+  (*           (* returnGen (UVALUE_I8 (repr x)) *) *)
+  (*       | 32%N => *)
+  (*           ret UVALUE_I32 <*> (returnGen repr <*> (choose (0, 2^32))) *)
+  (*           (* x <- choose (0, 2 ^ 32);; *) *)
+  (*           (* returnGen (UVALUE_I32 (repr x)) *) *)
+  (*       | 64%N => *)
+  (*           ret UVALUE_I64 <*> (returnGen repr <*> (choose (0, 2^64))) *)
+  (*           (* x <- choose (0, 2 ^ 63);; *) *)
+  (*           (* returnGen (UVALUE_I64 (repr x)) *) *)
+  (*       | _ => failGen "Invalid size" *)
+  (*       end *)
+  (*   | TYPE_Float => *)
+  (*       ret UVALUE_Float <*> fing32 *)
+  (*   | TYPE_Double => *)
+  (*       ret UVALUE_None (* FailGen *) *)
+  (*   | TYPE_Void => ret UVALUE_None *)
+  (*   | TYPE_Vector sz subtyp => *)
+  (*       ret UVALUE_Vector <*> vectorOf (N.to_nat sz) (gen_uvalue subtyp) *)
+  (*   | TYPE_Array sz subtyp => *)
+  (*       ret UVALUE_Array <*> vectorOf (N.to_nat sz) (gen_uvalue subtyp) *)
+  (*   | _ => failGen "Unimplemented uvalue generators" *)
+  (*   end. *)
   
 End GEN_ALIVE2.
 
-Module G := GEN_ALIVE2 MemoryModelImplementation.FinAddr MemoryModelImplementation.IP64Bit MemoryModelImplementation.FinSizeof LLVMEvents64.
+(* Module G := GEN_ALIVE2 MemoryModelImplementation.FinAddr MemoryModelImplementation.IP64Bit MemoryModelImplementation.FinSizeof  . (* LLVMEvents64. *) *)
  
 (* (* Extract Inlined Constant fst => "fst". *) *)
 (* (* Extract Inlined Constant app => "append". *) *)
